Almost prove soundness of Eval.

src/Eval.v
@@ -42,47 +42,47 @@ Fixpoint find_redex (e: expr) : (redex * expr_hole) + temp :=
   | expr_local x => inl (redex_local x, expr_hole_id)
 
   | expr_seq e1 e2 =>
-      match find_redex e1 with
-      | inl (r, ectx) => inl (r, expr_hole_seq ectx e2)
-      | inr t => inl (redex_seq t e2, expr_hole_id)
+      inl $ match find_redex e1 with
+      | inl (r, ectx) => (r, expr_hole_seq ectx e2)
+      | inr t => (redex_seq t e2, expr_hole_id)
       end
 
   | expr_recover e1 =>
-      match find_redex e1 with
-      | inl (r, ectx) => inl (r, expr_hole_recover ectx)
-      | inr t => inl (redex_recover t, expr_hole_id)
+      inl $ match find_redex e1 with
+      | inl (r, ectx) => (r, expr_hole_recover ectx)
+      | inr t => (redex_recover t, expr_hole_id)
       end
 
   | expr_assign_local x e1 =>
-      match find_redex e1 with
-      | inl (r, ectx) => inl (r, expr_hole_assign_local x ectx)
-      | inr t => inl (redex_assign_local x t, expr_hole_id)
+      inl $ match find_redex e1 with
+      | inl (r, ectx) => (r, expr_hole_assign_local x ectx)
+      | inr t => (redex_assign_local x t, expr_hole_id)
       end
 
   | expr_field e1 x =>
-      match find_redex e1 with
-      | inl (r, ectx) => inl (r, expr_hole_field ectx x)
-      | inr t => inl (redex_field t x, expr_hole_id)
+      inl $ match find_redex e1 with
+      | inl (r, ectx) => (r, expr_hole_field ectx x)
+      | inr t => (redex_field t x, expr_hole_id)
       end
 
   | expr_assign_field e1 x e2 =>
-      match find_redex e1, find_redex e2 with
-      | _, inl (r, ectx) => inl (r, expr_hole_assign_field1 e1 x ectx)
-      | inl (r, ectx), inr t2 => inl (r, expr_hole_assign_field2 ectx x t2)
-      | inr t1, inr t2 => inl (redex_assign_field t1 x t2, expr_hole_id)
+      inl $ match find_redex e1, find_redex e2 with
+      | _, inl (r, ectx) => (r, expr_hole_assign_field1 e1 x ectx)
+      | inl (r, ectx), inr t2 => (r, expr_hole_assign_field2 ectx x t2)
+      | inr t1, inr t2 => (redex_assign_field t1 x t2, expr_hole_id)
       end
 
   | expr_call e0 n es =>
-      match find_redex e0, list_find_redex es nil with
-      | _, inl (r, ts, ectx, es') => inl (r, expr_hole_call1 e0 n ts ectx es')
-      | inl (r, ectx), inr ts => inl (r, expr_hole_call2 ectx n ts)
-      | inr t0, inr ts => inl (redex_call t0 n ts, expr_hole_id)
+      inl $ match find_redex e0, list_find_redex es nil with
+      | _, inl (r, ts, ectx, es') => (r, expr_hole_call1 e0 n ts ectx es')
+      | inl (r, ectx), inr ts => (r, expr_hole_call2 ectx n ts)
+      | inr t0, inr ts => (redex_call t0 n ts, expr_hole_id)
       end
 
   | expr_ctor kt k es =>
-      match list_find_redex es nil with
-      | inl (r, ts, ectx, es') => inl (r, expr_hole_ctor kt k ts ectx es')
-      | inr ts => inl (redex_ctor kt k ts, expr_hole_id)
+      inl $ match list_find_redex es nil with
+      | inl (r, ts, ectx, es') => (r, expr_hole_ctor kt k ts ectx es')
+      | inr ts => (redex_ctor kt k ts, expr_hole_id)
       end
   end
 with 
@@ -97,27 +97,26 @@ with
   end
 .
 
-
-Definition eval (χ: heap) (σ: list frame) (e: expr) : option (heap * list frame * expr) :=
-  match find_redex e, σ with
-  | inl (redex_null, ectx), (φ::σ') =>
+Definition eval_redex (χ: heap) (σ: list frame) (r: redex) (ectx: expr_hole) : option (heap * list frame * expr) :=
+  match r, ectx, σ with
+  | redex_null, ectx, (φ::σ') =>
       let t := fresh φ in
       let φ' := <[t := v_null]>φ in
       Some (χ, φ'::σ', fill_hole ectx (expr_temp t))
 
-  | inl (redex_seq t e2, ectx), _ => Some (χ, σ, fill_hole ectx e2)
-  | inl (redex_recover t, ectx), _ => Some (χ, σ, fill_hole ectx (expr_temp t))
-  | inl (redex_local x, ectx), (φ::σ') =>
+  | redex_seq t e2, ectx, (φ::σ') => Some (χ, φ::σ', fill_hole ectx e2)
+  | redex_recover t, ectx, (φ::σ') => Some (χ, φ::σ', fill_hole ectx (expr_temp t))
+  | redex_local x, ectx, (φ::σ') =>
       let t := fresh φ in
       let φ' := <[t := φ !!! x]>φ in
       Some (χ, φ'::σ', fill_hole ectx (expr_temp t))
 
-  | inl (redex_assign_local x t, ectx), (φ::σ') =>
+  | redex_assign_local x t, ectx, (φ::σ') =>
       let t' := fresh φ in
       let φ' := <[t' := φ !!! x]>(<[x := φ !!! t]>φ) in
       Some (χ, φ'::σ', fill_hole ectx (expr_temp t'))
 
-  | inl (redex_field t x, ectx), (φ::σ') =>
+  | redex_field t x, ectx, (φ::σ') =>
       match φ !!! t with
       | v_null => Some (χ, φ::σ', fill_hole ectx (expr_temp t))
       | v_addr ω =>
@@ -126,7 +125,7 @@ Definition eval (χ: heap) (σ: list frame) (e: expr) : option (heap * list fram
           Some (χ, φ'::σ', fill_hole ectx (expr_temp t'))
       end
 
-  | inl (redex_assign_field t x t', ectx), (φ::σ') =>
+  | redex_assign_field t x t', ectx, (φ::σ') =>
       match φ !!! t with
       | v_null => Some (χ, φ::σ', fill_hole ectx (expr_temp t))
       | v_addr ω =>
@@ -136,7 +135,7 @@ Definition eval (χ: heap) (σ: list frame) (e: expr) : option (heap * list fram
           Some (χ', φ'::σ', fill_hole ectx (expr_temp t''))
       end
 
-  | inl (redex_call t0 n ts, ectx), (φ::σ') =>
+  | redex_call t0 n ts, ectx, (φ::σ') =>
       match φ !!! t0 with
       | v_addr ω => 
         obj <- χ !! ω;
@@ -156,10 +155,10 @@ Definition eval (χ: heap) (σ: list frame) (e: expr) : option (heap * list fram
 
         Some (χ, φ'' :: φ' :: σ', body)
 
-      | v_null => Some (χ, φ :: σ', expr_temp t0)
+      | v_null => Some (χ, φ :: σ', fill_hole ectx (expr_temp t0))
       end
 
-  | inl (redex_ctor kt k ts, ectx), (φ::σ') =>
+  | redex_ctor kt k ts, ectx, (φ::σ') =>
       fs <- lookup_Fs P kt;
       '(xs, body) <- lookup_Mr P kt k;
 
@@ -181,6 +180,20 @@ Definition eval (χ: heap) (σ: list frame) (e: expr) : option (heap * list fram
 
       Some (χ', φ'' :: φ' :: σ', body)
 
+  | redex_null, _, [] => None
+  | redex_seq _ _, _, [] => None
+  | redex_recover _, _, [] => None
+  | redex_local _, _, [] => None
+  | redex_assign_local _ _, _, [] => None
+  | redex_field _ _, _, [] => None
+  | redex_assign_field _ _ _, _, [] => None
+  | redex_call _ _ _, _, [] => None
+  | redex_ctor _ _ _, _, [] => None
+  end.
+
+Definition eval (χ: heap) (σ: list frame) (e: expr) : option (heap * list frame * expr) :=
+  match find_redex e, σ with
+  | inl (r, ectx), σ => eval_redex χ σ r ectx
   | inr t, (φ'::φ::σ') =>
       let t' := fresh φ in
       let φ'' := {|
@@ -188,17 +201,260 @@ Definition eval (χ: heap) (σ: list frame) (e: expr) : option (heap * list fram
           locals := <[ t' := φ' !!! t ]>φ.(locals);
           hole := expr_hole_id
       |} in
-      
+
       Some (χ, φ'' :: σ', fill_hole φ.(hole) (expr_temp t'))
 
-  | inl (redex_null, _), [] => None
-  | inl (redex_local _, _), [] => None
-  | inl (redex_assign_local _ _, _), [] => None
-  | inl (redex_field _ _, _), [] => None
-  | inl (redex_assign_field _ _ _, _), [] => None
-  | inl (redex_call _ _ _, _), [] => None
-  | inl (redex_ctor _ _ _, _), [] => None
   | inr _, [] => None
   | inr _, [_] => None
   end.
 End eval.
+
+Definition expr_redex (r: redex) : expr :=
+  match r with
+  | redex_null => expr_null
+  | redex_seq t e2 => expr_seq (expr_temp t) e2
+  | redex_recover t => expr_recover (expr_temp t)
+  | redex_local x => expr_local x
+  | redex_assign_local x t => expr_assign_local x (expr_temp t)
+  | redex_field t f => expr_field (expr_temp t) f
+  | redex_assign_field t0 f t1 => expr_assign_field (expr_temp t0) f (expr_temp t1)
+  | redex_call t0 n ts => expr_call (expr_temp t0) n (list_expr_temps ts)
+  | redex_ctor kt k ts => expr_ctor kt k (list_expr_temps ts)
+  end.
+
+Lemma find_redex_fill : forall e e' r ectx,
+  find_redex e = inl (r, ectx) ->
+  e' = expr_redex r ->
+  e = fill_hole ectx (e').
+Proof.
+Admitted.
+
+Lemma eval_redex_sound : forall P χ χ' σ σ' ectx r e e',
+  find_redex e = inl (r, ectx) ->
+  eval_redex P χ σ r ectx = Some (χ', σ', e') -> step P (χ, σ, e) (χ', σ', e').
+Proof.
+intros.
+destruct σ.
+unfold eval_redex in  H0.
+destruct r.
+inversion H0.
+inversion H0.
+inversion H0.
+inversion H0.
+inversion H0.
+inversion H0.
+inversion H0.
+inversion H0.
+inversion H0.
+
+remember r as r0.
+destruct r.
+unfold eval_redex in H0.
+rewrite Heqr0 in H0.
+inversion H0.
+assert (e = fill_hole ectx (expr_redex r0)).
+apply find_redex_fill with r0.
+exact H.
+reflexivity.
+rewrite H1.
+rewrite Heqr0.
+unfold expr_redex.
+apply step_hole.
+apply step_null.
+admit.
+reflexivity.
+
+unfold eval_redex in H0.
+rewrite Heqr0 in H0.
+inversion H0.
+assert (e = fill_hole ectx (expr_redex r0)).
+apply find_redex_fill with r0.
+exact H.
+reflexivity.
+rewrite H1.
+rewrite Heqr0.
+unfold expr_redex.
+apply step_hole.
+apply step_seq.
+
+unfold eval_redex in H0.
+rewrite Heqr0 in H0.
+inversion H0.
+assert (e = fill_hole ectx (expr_redex r0)).
+apply find_redex_fill with r0.
+exact H.
+reflexivity.
+rewrite H1.
+rewrite Heqr0.
+unfold expr_redex.
+apply step_hole.
+apply step_recover.
+
+unfold eval_redex in H0.
+rewrite Heqr0 in H0.
+inversion H0.
+assert (e = fill_hole ectx (expr_redex r0)).
+apply find_redex_fill with r0.
+exact H.
+reflexivity.
+rewrite H1.
+rewrite Heqr0.
+unfold expr_redex.
+apply step_hole.
+apply step_local.
+admit.
+reflexivity.
+
+unfold eval_redex in H0.
+rewrite Heqr0 in H0.
+inversion H0.
+assert (e = fill_hole ectx (expr_redex r0)).
+apply find_redex_fill with r0.
+exact H.
+reflexivity.
+rewrite H1.
+rewrite Heqr0.
+unfold expr_redex.
+apply step_hole.
+apply step_asn_local.
+admit.
+reflexivity.
+
+unfold eval_redex in H0.
+rewrite Heqr0 in H0.
+assert (e = fill_hole ectx (expr_redex r0)).
+apply find_redex_fill with r0.
+exact H.
+reflexivity.
+rewrite H1.
+rewrite Heqr0.
+unfold expr_redex.
+destruct (f !!! t) eqn:?.
+inversion H0.
+apply step_hole.
+apply step_field_null.
+symmetry.
+exact Heqy.
+inversion H0.
+apply step_hole.
+apply step_field with a.
+admit.
+symmetry.
+exact Heqy.
+reflexivity.
+
+unfold eval_redex in H0.
+rewrite Heqr0 in H0.
+assert (e = fill_hole ectx (expr_redex r0)).
+apply find_redex_fill with r0.
+exact H.
+reflexivity.
+rewrite H1.
+rewrite Heqr0.
+unfold expr_redex.
+destruct (f !!! t) eqn:?.
+inversion H0.
+apply step_hole.
+apply step_asn_field_null.
+symmetry.
+exact Heqy.
+inversion H0.
+apply step_hole.
+apply step_asn_field with a.
+admit.
+symmetry.
+exact Heqy.
+reflexivity.
+reflexivity.
+
+unfold eval_redex in H0.
+rewrite Heqr0 in H0.
+assert (e = fill_hole ectx (expr_redex r0)).
+apply find_redex_fill with r0.
+exact H.
+reflexivity.
+rewrite H1. rewrite Heqr0.
+unfold expr_redex.
+destruct (f !!! t) eqn:?.
+inversion H0.
+apply step_hole.
+apply step_call_null.
+auto.
+destruct (χ !! a) eqn:?. simpl in H0.
+destruct (lookup_Mr P (name o) s) eqn:?.
+simpl in H0.
+destruct p as [xs body].
+inversion H0.
+apply step_sync with xs a.
+symmetry.
+exact Heqy.
+rewrite <- H3. rewrite Heqo.
+simpl.
+symmetry. rewrite <- H5. exact Heqo0.
+reflexivity.
+reflexivity.
+simpl in H0. inversion H0.
+simpl in H0. inversion H0.
+
+unfold eval_redex in H0.
+rewrite Heqr0 in H0.
+assert (e = fill_hole ectx (expr_redex r0)).
+apply find_redex_fill with r0.
+auto with *.
+auto with *.
+rewrite H1.
+rewrite Heqr0.
+unfold expr_redex.
+destruct (lookup_Fs P s) as [fs|] eqn:?. simpl in H0.
+destruct (lookup_Mr P s s0) eqn:?. simpl in H0.
+destruct p as [xs body].
+inversion H0.
+apply step_ctor with (Nfresh χ) fs xs.
+
+apply fin_map_dom.not_elem_of_dom.
+apply Nfresh_fresh.
+auto with *.
+auto with *.
+auto with *.
+auto with *.
+auto with *.
+simpl in H0. inversion H0.
+simpl in H0. inversion H0.
+
+Admitted.
+
+Lemma eval_sound : forall P χ χ' σ σ' e e',
+  eval P χ σ e = Some (χ', σ', e') -> step P (χ, σ, e) (χ', σ', e').
+Proof.
+intros.
+unfold eval in H.
+destruct (find_redex e) eqn:?.
+destruct p.
+apply eval_redex_sound with (P:=P) (r:=r) (ectx:=e0).
+exact Heqs.
+exact H.
+
+assert (e = expr_temp t).
+destruct e.
+unfold find_redex in Heqs. inversion Heqs. reflexivity.
+
+unfold find_redex in Heqs. inversion Heqs.
+unfold find_redex in Heqs. inversion Heqs.
+unfold find_redex in Heqs. inversion Heqs.
+unfold find_redex in Heqs. inversion Heqs.
+unfold find_redex in Heqs. inversion Heqs.
+unfold find_redex in Heqs. inversion Heqs.
+unfold find_redex in Heqs. inversion Heqs.
+unfold find_redex in Heqs. inversion Heqs.
+unfold find_redex in Heqs. inversion Heqs.
+
+destruct σ.
+inversion H.
+destruct σ.
+inversion H.
+inversion H.
+rewrite H0.
+apply step_return.
+admit.
+reflexivity.
+Admitted.
